\documentclass[newpage,hints,handout]{ximera}

\input{../preamble.tex}

\title{Central projection}
\begin{document}
\begin{abstract}
Here we start to develop unified models for our geometries.
\end{abstract}
\maketitle

\section{Central projection coordinates}

Now we will examine one way to produce coordinates uniformly for spherical, plane, and hyperbolic geometry that will allow us to pass smoothly through the three geometries. Let's project $K$-geometry,
\[
1=K\left(x^{2}+y^{2}\right)+z^{2} 
\]
onto the plane $z=1$ using the origin $O=(0,0,0)$ as the center of
projection:
\begin{image}
\includegraphics[width=5in]{KGeomCentralProjection.png}
\end{image}
Let's look at this from a different vantage point, say with our eye
along the edge of the plane $z=1$:
\begin{image}
\includegraphics[width=5in]{2dCentralProjection.png}
\end{image}
Note, we are only projecting the top of the surface
\[
1=K\left(x^{2}+y^{2}\right)+z^{2} 
\]
onto the plane $z=1$. So when $K>0$, this is the ``Northern hemisphere'' of
the sphere, when $K<0$, this is the upper hyperboloid, and when $K=0$,
this is the plane $z=1$.

\begin{problem}
  Use similar triangles to explain why for any given $(x,y,z)$, there
  is a number $\lambda$ such that
  \[
  \lambda\cdot(x_c,y_c,1) = (x,y,z).
  \]
  \begin{freeResponse}
    Let $A = (x,y,z)$, $B= (x,y,0)$, $A_c = (x_c,y_c,1)$ and
    $B_c=(x_c,y_c,0)$. From the diagram above we see that
    \[
    \angle AOB = \angle A_c O B_c.
    \]
    Moreover, since $\triangle AOB$ and $\triangle A_c O B_c$ are
    right triangles, we now see that two of their angles have the same
    measure, and hence all three have the same measure. This means
    that these triangles are similar, and hence there they are
    dilations of one another. Hence there is a scale-factor $\lambda$
    such that
    \[
    \lambda\cdot(x_c,y_c,1) = (x,y,z).
    \]
  \end{freeResponse}
\end{problem}


\begin{problem}
  What range of values could $\lambda$ take when $K>0$?
  \begin{freeResponse}
    In this case, $\lambda\in (0,1]$.
  \end{freeResponse}
\end{problem}

\begin{problem}
  What range of values could $\lambda$ take when $K<0$?
  \begin{freeResponse}
    In this case, $\lambda\in[1,\infty)$.
  \end{freeResponse}
\end{problem}

\begin{problem}
  What range of values could $\lambda$ take when $K=0$?
  \begin{freeResponse}
    In this case
    \[
    1=K\left(x^{2}+y^{2}\right)+z^{2} 
    \]
    is the plane $z = 1$, hence $\lambda=1$.
  \end{freeResponse}
\end{problem}



\begin{problem}
  For the projection of the set $1=K\left(x^{2}+y^{2}\right)+z^{2}$
  onto the $z=1$ plane with center of projection $O$, write
  $(x_{c},y_{c})$ as a function of $(x,y,z)$.
  \begin{freeResponse}
    We know that
    \[
    \lambda\cdot(x_{c},y_{c},1)=(x,y,z),
    \]
    hence $\lambda=z$, and we may now write
    \begin{align*}
      x_{c} &=x/z,\\
      y_{c} &=y/z.
    \end{align*}
  \end{freeResponse}
\end{problem}

\begin{problem}
  For the projection of the set $1=K\left(x^{2}+y^{2}\right)+z^{2} $
  onto the $z=1$ plane with center of projection $O$, write $(x,y,z)$
  as a function of $(x_{c},y_{c})$.
  \begin{freeResponse}
    This is slightly more complex than the previous problem; however,
    we will begin the same way. We know that
    \[
    \lambda\cdot(x_{c},y_{c},1)=(x,y,z),
    \]
    hence $\lambda=z$, and we may now write
    \begin{align*}
      x &= x_c\cdot z,\\
      y &= y_c\cdot z,\\
      z &= z.
    \end{align*}
    Now our task is to write $z$ in terms of $x_c$ and $y_c$. Using our assignments above, write
    \begin{align*}
      1 &= K\left(x^2 + y^2\right) + z^2\\
      1 &= K\left((x_c\cdot z)^2 + (y_c\cdot z)^2\right) + z^2\\
      1 &= \left(K\left(x_c^2 + y_c^2\right)+1\right)z^2,
    \end{align*}
    and so
    \[
    z = \frac{1}{\sqrt{K\left(x_c^2 + y_c^2\right)+1}}.
    \]
    Hence
    \begin{align*}
      x &= \frac{x_c}{\sqrt{K\left(x_c^2 + y_c^2\right)+1}},\\
      y &= \frac{y_c}{\sqrt{K\left(x_c^2 + y_c^2\right)+1}},\\
      z &= \frac{1}{\sqrt{K\left(x_c^2 + y_c^2\right)+1}}.\\
    \end{align*}
  \end{freeResponse}
\end{problem}






\section{Central projection dot product}

Like we have done before, now we want to be able to find a dot product
that will allow us to compute lengths in central projection
coordinates that will agree with the $K$-dot product, and hence the
euclidean dot product.


\begin{problem}
Suppose we have a curve $\gamma$ in $K$-warped space which we can decompose as
\[
\xymatrix{
  t \ar@{|->}[r]^-{\gamma_{c}} \ar@{|->}@/_1pc/[rr]_{\gamma} & (x_c(t),y_c(t)) \ar@{|->}[r]^-{\left[\begin{smallmatrix}x(x_c,y_c)\\y(x_c,y_c)\\z(x_c,y_c)\end{smallmatrix}\right]} & \gamma(t)=(x(t),y(t),z(t))
}
\]
Use the chain rule to compute
\[
\dd[x]{t}, \qquad \dd[y]{t}, \qquad \dd[z]{t},
\]
in terms of $\dd[x_c]{t}$, $\dd[y_c]{t}$, $\pp[x]{x_c}$,
$\pp[y]{x_c}$, $\pp[z]{x_c}$, $\pp[x]{y_c}$, $\pp[y]{y_c}$,
and $\pp[z]{y_c}$.
  \begin{hint}
  Simply write down the answer from a previous problem with some minor
  changes.
  \end{hint}
  \begin{freeResponse}
  Write
  \begin{align*}
    \dd[x]{t} &= \begin{bmatrix}\pp[x]{x_c} & \pp[x]{y_c}\end{bmatrix}\cdot\begin{bmatrix}\dd[x_c]{t} & \dd[y_c]{t}\end{bmatrix}^\transpose = \pp[x]{x_c}\cdot\dd[x_c]{t}+\pp[x]{y_c}\cdot\dd[y_c]{t},   \\
    \dd[y]{t} &= \begin{bmatrix}\pp[y]{x_c} & \pp[y]{y_c}\end{bmatrix}\cdot\begin{bmatrix}\dd[x_c]{t} & \dd[y_c]{t}\end{bmatrix}^\transpose = \pp[y]{x_c}\cdot\dd[x_c]{t}+\pp[y]{y_c}\cdot\dd[y_c]{t},   \\
    \dd[z]{t} &= \begin{bmatrix}\pp[z]{x_c} & \pp[z]{y_c}\end{bmatrix}\cdot\begin{bmatrix}\dd[x_c]{t} & \dd[y_c]{t}\end{bmatrix}^\transpose = \pp[z]{x_c}\cdot\dd[x_c]{t}+\pp[z]{y_c}\cdot\dd[y_c]{t}.  
  \end{align*}
\end{freeResponse}
\end{problem}




\begin{problem}
  With the same setting as in the previous problem, rewrite the result
  of your computation in matrix notation to find $D_c$ such that
  \[
  \begin{bmatrix}
    dx/dt \\ dy/dt \\ dz/dt
  \end{bmatrix}
  =D_c \cdot
  \begin{bmatrix}
    dx_c/dt \\ dy_c/dt
  \end{bmatrix}
  \]
  in terms of $\pp[x]{x_c}$, $\pp[y]{x_c}$, $\pp[z]{x_c}$,
  $\pp[x]{y_c}$, $\pp[y]{y_c}$, and $\pp[z]{y_c}$.
  \begin{hint}
    Simply write down the answer from a previous problem with some minor
    changes.
  \end{hint}
  \begin{freeResponse}
    \[
    D_c =
    \begin{bmatrix}
      \pp[x]{x_c} & \pp[y]{x_c} & \pp[z]{x_c} \\
      \pp[x]{y_c}   & \pp[y]{y_c}   & \pp[z]{y_c}
    \end{bmatrix}.
    \]
  \end{freeResponse}
\end{problem}




\begin{problem}
  Now find $P_c$ in terms of $K$, $\pp[x]{x_c}$, $\pp[y]{x_c}$,
  $\pp[z]{x_c}$, $\pp[x]{y_c}$, $\pp[y]{y_c}$, and $\pp[z]{y_c}$ such
  that
  \[
  \left(\dd[x]{t}, \dd[y]{t}, \dd[z]{t}\right)\bullet_K
  \left(\dd[x]{t}, \dd[y]{t}, \dd[z]{t}\right)
  =
  \begin{bmatrix}
    \dd[x_c]{t} &  \dd[y_c]{t}
  \end{bmatrix}
  \cdot P_c
  \cdot
  \begin{bmatrix}
    \dd[x_c]{t} \\  \dd[y_c]{t}
  \end{bmatrix}.
  \]
  \begin{hint}
  Simply write down the answer from a previous problem with some minor
  changes.
  \end{hint}
  \begin{freeResponse}
    For completeness sake, we will include a complete solution.
    Working from the $K$-dot product, we need that
    \begin{align*}
    \left(\dd[x]{t}, \dd[y]{t}, \dd[z]{t}\right)\bullet_K
    \left(\dd[x]{t}, \dd[y]{t}, \dd[z]{t}\right)
    &=
    \begin{bmatrix}
      \dd[x]{t} & \dd[y]{t} & \dd[z]{t}
    \end{bmatrix}
    \begin{bmatrix}
      1 & 0 & 0\\
      0 & 1 & 0\\
      0 & 0 & K^{-1}
    \end{bmatrix}
    \begin{bmatrix}
      \dd[x]{t} \\ \dd[y]{t} \\ \dd[z]{t}
    \end{bmatrix}\\
    &=
    \begin{bmatrix}
      \frac{dx_c}{dt} & \frac{dy_c}{dt}
    \end{bmatrix}\cdot D_{c}\cdot
    \begin{bmatrix}
      1 & 0 & 0\\
      0 & 1 & 0\\
    0 & 0 & K^{-1}
    \end{bmatrix}
    \cdot
    \left(
    \begin{bmatrix}
      \frac{dx_c}{dt} & \frac{dy_c}{dt}
    \end{bmatrix}\cdot D_{c}
    \right)^\transpose\\
    &=
    \begin{bmatrix}
      \frac{dx_c}{dt} & \frac{dy_c}{dt}
    \end{bmatrix}\cdot D_{c}\cdot
    \begin{bmatrix}
      1 & 0 & 0\\
      0 & 1 & 0\\
    0 & 0 & K^{-1}
    \end{bmatrix}
    \cdot
    D_{c}^\transpose
    \cdot \begin{bmatrix}
      \frac{dx_c}{dt} \\ \frac{dy_c}{dt}
    \end{bmatrix}.
  \end{align*}
    Hence
    \begin{align*}
      P_c &=
      \begin{bmatrix}
        \pp[x]{x_c} & \pp[y]{x_c} & \pp[z]{x_c} \\
        \pp[x]{y_c} & \pp[y]{y_c} & \pp[z]{y_c}
      \end{bmatrix}
      \begin{bmatrix}
        1 & 0 & 0\\
        0 & 1 & 0\\
        0 & 0 & K^{-1}
      \end{bmatrix}
      \begin{bmatrix}
        \pp[x]{x_c} & \pp[x]{y_c}\\ 
        \pp[y]{x_c} & \pp[y]{y_c}\\
        \pp[z]{x_c} & \pp[z]{y_c}
      \end{bmatrix}\\
      &=
      \begin{bmatrix}
        \left(\pp[x]{x_c}\right)^2 + \left(\pp[y]{x_c}\right)^2 + \left(\pp[z]{x_c}\right)^2K^{-1} & \pp[x]{x_c}\pp[x]{y_c} + \pp[y]{x_c}\pp[y]{y_c} + \pp[z]{x_c}\pp[z]{y_c} K^{-1}\\
        \pp[x]{x_c}\pp[x]{y_c} + \pp[y]{x_c}\pp[y]{y_c} + \pp[z]{x_c}\pp[z]{y_c} K^{-1}       & \left(\pp[x]{y_c}\right)^2 + \left(\pp[y]{y_c}\right)^2 + \left(\pp[z]{y_c}\right)^2K^{-1}
      \end{bmatrix}.
    \end{align*}
  \end{freeResponse}
\end{problem}

Before we actually compute $P_c$, it will help to compute the partial
derivatives.

\begin{problem}
  Set
  \begin{align*}
    x(x_c,y_c) &=\lambda\cdot x_c,\\
    y(x_c,y_c) &=\lambda\cdot y_c,\\
    z(x_c,y_c) &=\lambda,
  \end{align*}
  and show that
  \[
  \begin{split}
    \pp[x]{x_c} &=\lambda -Kx_c^2 \lambda^3,\\
    \pp[y]{x_c} &=-Kx_cy_c \lambda^3,\\
    \pp[z]{x_c} &=-Kx_c \lambda^3,
  \end{split}
  \qquad
  \begin{split}
    \pp[x]{y_c} &= -Kx_cy_c \lambda^3,\\
    \pp[y]{y_c} &= \lambda - Ky_c^2 \lambda^3,\\
    \pp[z]{y_c} &= -Ky_c \lambda^3.
  \end{split}
  \]
  \begin{hint}
  Work in the following way:
  \begin{enumerate}
  \item Remember that $\lambda$ is itself a function of $x_c$ and $y_c$, so its
    partial derivatives also matter.  Use the product rule:
    $$\pp[x]{x_c} = \lambda + x_c \cdot \pp[\lambda]{x_c}.$$
  \item Express the partial derivative in terms of $\lambda$, $K$, $x_c$, and
    $y_c$.
  \end{enumerate}
\end{hint}
  \begin{freeResponse}
    Write
  \begin{align*}
    \pp[x]{x_c} &= \lambda  + x_c \cdot \pp[\lambda]{x_c}\\
    &= \lambda + x_c \cdot \pp{x_c} \left(K\left(x_c^2 + y_c^2\right)+1\right)^{-1/2}\\
    &= \lambda + x_c \cdot (-1/2)\left(K\left(x_c^2 + y_c^2\right)+1\right)^{-3/2}(2Kx_c)\\
    &= \lambda -Kx_c^2 \lambda^3.
  \end{align*}
  Similarly,
    \begin{align*}
    \pp[y]{x_c} &= y_c \cdot \pp[\lambda]{x_c}\\
    &= y_c \cdot \pp{x_c} \left(K\left(x_c^2 + y_c^2\right)+1\right)^{-1/2}\\
    &= y_c \cdot (-1/2)\left(K\left(x_c^2 + y_c^2\right)+1\right)^{-3/2}(2Kx_c)\\
    &= -Kx_cy_c \lambda^3.
    \end{align*}
   Finally, 
    \begin{align*}
    \pp[z]{x_c} &= \pp[\lambda]{x_c}\\
    &= \pp{x_c}\left(K\left(x_c^2 + y_c^2\right)+1\right)^{-1/2}\\
    &= (-1/2)\left(K\left(x_c^2 + y_c^2\right)+1\right)^{-3/2}(2Kx_c)\\
    &= -Kx_c \lambda^3.
    \end{align*}
    Now with entirely similar computations, we see
    \begin{align*}
      \pp[x]{y_c} &= -Kx_cy_c \lambda^3,\\
      \pp[y]{y_c} &= \lambda - Ky_c^2 \lambda^3,\\
      \pp[z]{y_c} &= -Ky_c \lambda^3.
    \end{align*}
  \end{freeResponse}
\end{problem}



\begin{problem}
With the same setting as above, show that $P_c$ is
  \[
  P_c =
  \begin{bmatrix}
    \left(Ky_c^2+1\right)\lambda^4 & -Kx_{c}y_{c}\lambda^4\\
    -Kx_{c}y_{c}\lambda^4 & \left(Kx_c^2+1\right)\lambda^4
  \end{bmatrix}.
\]

\begin{hint}
  When simplifying, combine the terms with the highest degree of $\lambda$
  and note that
  \[
  \lambda^{-2} = K\left(x_c^2 + y_c^2\right) + 1.
  \]
\end{hint}
\begin{freeResponse}
  
  Write $\left(\pp[x]{x_c}\right)^2 + \left(\pp[y]{x_c}\right)^2 +\left(\pp[z]{x_c}\right)^2K^{-1}$
    \begin{align*}
      &= \left(\lambda -Kx_c^2 \lambda^3\right)^2 + \left(-Kx_cy_c \lambda^3\right)^2 + \left(-Kx_c \lambda^3\right)^2K^{-1}\\
      &= \lambda^2 - 2Kx_c^2\lambda^4 + K^2x_c^4 \lambda^6+ K^2x_c^2y_c^2\lambda^6 + Kx_c^2\lambda^6\\
      &= \lambda^2 - 2Kx_c^2\lambda^4 + Kx_c^2\lambda^6\left(Kx_c^2 + Ky_c^2 + 1\right)\\
      &= \lambda^2 - 2Kx_c^2\lambda^4 + Kx_c^2\lambda^6\left(K\left(x_c^2 + y_c^2\right) + 1\right)\\
      &= \lambda^2 - 2Kx_c^2\lambda^4 + Kx_c^2\lambda^6 \lambda^{-2}\\
      &= \lambda^2 - 2Kx_c^2\lambda^4 + Kx_c^2\lambda^4\\
      &= \lambda^2 - Kx_c^2\lambda^4\\
      &= \frac{1}{K\left(x_c^2+y_c^2\right)+1} - \frac{Kx_c^2}{\left(K\left(x_c^2+y_c^2\right)+1\right)^2}\\
      &= \frac{K\left(x_c^2 + y_c^2\right) +1 - Kx_c^2}{\left(K\left(x_c^2+y_c^2\right)+1\right)^2}\\
      &= \frac{Ky_c^2+1}{\left(K\left(x_c^2+y_c^2\right)+1\right)^2}\\
      &= \left(Ky_c^2+1\right)\lambda^4.
    \end{align*}
    
    That $\pp[x]{x_c}\pp[x]{y_c} + \pp[y]{x_c}\pp[y]{y_c} + \pp[z]{x_c}\pp[z]{y_c} K^{-1}$
    \begin{align*}
      &=\left(\lambda -Kx_c^2 \lambda^3\right)\left(-Kx_cy_c \lambda^3\right) + \left(-Kx_cy_c \lambda^3\right)\left(\lambda - Ky_c^2 \lambda^3\right) + \left(-Kx_c \lambda^3\right)\left(-Ky_c \lambda^3\right)K^{-1}\\
      &= -Kx_cy_c\lambda^4+K^2x_c^3y_c\lambda^6-Kx_cy_c\lambda^4+K^2x_cy_c^3\lambda^6+Kx_cy_c\lambda^6\\
      &= K^2x_c^3y_c\lambda^6+K^2x_cy_c^3\lambda^6+Kx_cy_c\lambda^6 -2Kx_cy_c\lambda^4\\
      &= Kx_cy_c\lambda^6\left(K\left(x_c^2 + y_c^2\right) + 1\right)-2Kx_cy_c\lambda^4\\
      &= Kx_cy_c\lambda^6\lambda^{-2} -2Kx_cy_c\lambda^4\\
      &= Kx_cy_c\lambda^4 -2Kx_cy_c\lambda^4\\
      &= -Kx_cy_c\lambda^4.
    \end{align*}
    With entirely analogous computations, we see that 
    \[
     P_c =
     \begin{bmatrix}
       \left(Ky_c^2+1\right)\lambda^4 & -Kx_{c}y_{c}\lambda^4\\
       -Kx_{c}y_{c}\lambda^4 & \left(Kx_c^2+1\right)\lambda^4
     \end{bmatrix}.
     \]
  \end{freeResponse}
\end{problem}


\begin{definition}
  Let $\mathbf{v}_c$ and $\mathbf{w}_c$ be vectors in $(x_c,y_c)$-coordinates
  originating at the same $(x_c,y_c)$-coordinate. Define
  \[
  \mathbf{v}_c \bullet_c \mathbf{w}_c = \mathbf{v}_c^\transpose P_c \mathbf{w}_c
  \]
  where
  \[
  P_c =
  \begin{bmatrix}
    \left(Ky_c^2+1\right)\lambda^4 & -Kx_{c}y_{c}\lambda^4\\
    -Kx_{c}y_{c}\lambda^4 & \left(Kx_c^2+1\right)\lambda^4
  \end{bmatrix}
  \]
  and $\lambda$, $x_c$, and $y_c$ are determined by the
  coordinate that the vectors originate from.
\end{definition}


\section{When the finite is infinite and the infinite is finite}

Central projection allows us to think about both ``finite'' areas and
``infinite'' areas in new ways.

\paragraph{When $K$ is positive, the finite is infinite}

When $K>0$, we are working with a sphere. As we know, a sphere has
finite surface area.

\begin{problem}
  As a point approaches the equator of the $R$-sphere from the North
  Pole, where does it move to under central projection?
  \begin{hint}
    A picture is worth a thousand words!
  \end{hint}
  \begin{freeResponse}
  %centralProjectionSpherical geogebra
  As a point approaches the equator of the $R$-sphere, its image in central projection approaches infinity. 
  \end{freeResponse}
\end{problem}

\begin{problem}
  Explain why one might say that central projection makes the
  ``finite'' seem ``infinite.''
    \begin{freeResponse}
    The surface area of sphere is finite, but its image in central projection is a plane with infinite surface area. Also, the distance a point travels along a line away from the north pole has a finite maximum distance as it approaches the equator. However, the distance from the image of the point in central projection to the origin goes to infinity. 
    \end{freeResponse}
\end{problem}


\paragraph{When $K$ is negative, the infinite is finite}


Notice that, if $K<0$, the equation for the $K$-plane becomes
\[
z^{2}-|K|(x^{2}+y^2)  =1.
\]
This describes a $2$-sheeted hyperboloid with the $z$-axis as major axis.  We
will only consider the sheet on which $z$ is positive as forming the
$K$-geometry. In plain English, this means we are doing geometry on this
hyperboloid:
\begin{image}
\includegraphics[width=3in]{UpperHyperboloid.png}
\end{image}
Of critical importance, note

\begin{center}
  \textbf{this hyperboloid has infinite surface area.}
\end{center}

The hyperboloid above is obtained by rotating the hyperbola
\[
z^{2}-\left\vert K\right\vert x^{2}= 1
\]
in the $(x,z)$-plane around the $z$-axis.
\begin{image}
\includegraphics[width=3in]{UpperHyperbola.png}
\end{image}


\begin{problem}
  Consider points of the form $(x,0,z)$ in $K$-geometry.  As $x$ and $z$ shoot
  off to infinity, what happens to the corresponding central projection
  coordinate $x_c$?  Relate this to the asymptote of the hyperbola as
  $x \to \infty$.
  \begin{hint}
    First rewrite $z^{2}-|K|x^{2} =1$ as
    \[
    z = \sqrt{1+|K|x^2}
    \]
    and explain why this is acceptable.
  \end{hint}
  \begin{hint}
    Explain why computing this limit
    \[
    \lim_{x\to \infty} \frac{\sqrt{1+|K|x^2}}{x}
    \]
    helps us in this context.
  \end{hint}
  \begin{freeResponse}
    Since we are only considering the upper hyperboloid, we need only
    look at the upper hyperbola. Hence we may look at
     \[
    z = \sqrt{1+|K|x^2}.
    \]
    To compute the maximum distance the image of a point can be from
    the origin, look at 
    \[
    \lim_{x\to \infty} \frac{\sqrt{1+|K|x^2}}{x}
    \]
    as this computes the ``end-behavior'' of the ``slope'' of the
    curve. Write
    \begin{align*}
      \lim_{x\to \infty} \frac{\sqrt{1+|K|x^2}}{x} &= \lim_{x\to \infty} \frac{\sqrt{1+|K|x^2}}{x}\cdot \frac{1/x}{1/x}\\
      &= \lim_{x\to \infty} \sqrt{1/x^2+|K|}\\
      &= \sqrt{|K|}.
    \end{align*}
    Hence the equation of the line is given by $z = x\sqrt{|K|}$.
  \end{freeResponse}
\end{problem}

\begin{problem}
  When $K<0$, what is the set of points $(x_c,y_c)$ in central projection which
  correspond to points on the hyperboloid?
  \begin{hint}
    Use the answer to the previous question and the fact that both the
    hyperboloid and the process of central projection are symmetric with respect
    to rotation around the $z$-axis.
  \end{hint}
  \begin{freeResponse}
    We must find where $z = x\sqrt{|K|}$ intersects the line $z=1$. To do this, simply solve
    \[
    1 = x\sqrt{|K|}
    \]
    for $x$, and so the radius is $1/\sqrt{|K|}$.
  \end{freeResponse}
\end{problem}

\begin{problem}
  Explain why one might say that central projection makes the
  ``infinite'' seem ``finite.''
    \begin{freeResponse}
    As a point in $K$-geometry goes to infinity, its $K$-distance from the origin goes to infinity. However, the image of the point in central projection is bounded by the circle of radius $\frac{1}{\sqrt{K}}$. Therefore, the distance from the point in central projection to the origin appears to be less than $\frac{1}{\sqrt{K}}$.
    \end{freeResponse}
\end{problem}

The $(x_{c},y_{c})$-coordinates are called \dfn{Klein coordinates} for
hyperbolic geometry and the disk of radius $1/\sqrt{|K|}$ called the
\dfn{Klein model} for hyperbolic geometry in honor of the famous
German geometer, Felix Klein.

\begin{problem}
Summarize the results from this section. In particular, indicate which
results follow from the others.
\begin{freeResponse}
\end{freeResponse}
\end{problem}


\end{document}
